aarch64 crefine: introduce pt_array_relation
The retype annotations in C for page tables are array annotations. This
conflicts with our previous strategy of avoiding arrays for page tables
in C. We can't change the annotations, because we access PTEs with
pointer arithmetic, which does generate array assertions, which in turn
can only be satisfied if there are array type tags in the heap.

We can re-use the cvariable_array_map_relation from CNodes for the new
pt_array_relation at the cost of new sorries and requiring new
assertions in Haskell.

Signed-off-by: Gerwin Klein <gerwin.klein@proofcraft.systems>

proof/crefine/AARCH64/Retype_C.thy
@@ -1949,10 +1949,10 @@ lemma cmap_relation_array_add_array[OF refl]:
   apply (rule shiftl_less_t2n, rule word_of_nat_less, simp_all add: word_bits_def)
   done
 
-(* FIXME AARCH64 the pt_t being a free var is probably not what we want, the 512 magic number is
-   not clear in this case (9 bits \<rightarrow> 512 PTEs in a PT on RISCV64?) *)
-lemma createObjects_ccorres_pte:
+lemma createObjects_ccorres_pte_pt:
   defines "ko \<equiv> (KOArch (KOPTE (makeObject :: pte)))"
+  (* unfortunately, because of the pt_Ptr in ptr_retyps below, we can't make this lemma generic *)
+  defines "pt_t \<equiv> NormalPT_T"
   shows "\<forall>\<sigma> x. (\<sigma>, x) \<in> rf_sr \<and> ptr \<noteq> 0
   \<and> pspace_aligned' \<sigma> \<and> pspace_distinct' \<sigma>
   \<and> pspace_no_overlap' ptr sz \<sigma>
@@ -1961,18 +1961,22 @@ lemma createObjects_ccorres_pte:
   \<and> range_cover ptr sz (ptBits pt_t) 1
   \<and> valid_global_refs' s
   \<and> kernel_data_refs \<inter> {ptr..+ 2 ^ (ptBits pt_t) } = {} \<longrightarrow>
-  (\<sigma>\<lparr>ksPSpace := foldr (\<lambda>addr. data_map_insert addr ko) (new_cap_addrs 512 ptr ko) (ksPSpace \<sigma>)\<rparr>,
+  (\<sigma>\<lparr>ksPSpace := foldr (\<lambda>addr. data_map_insert addr ko)
+                       (new_cap_addrs (2 ^ (ptTranslationBits pt_t)) ptr ko) (ksPSpace \<sigma>)\<rparr>,
    x\<lparr>globals := globals x
                  \<lparr>t_hrs_' := hrs_htd_update (ptr_retyps_gen 1 (pt_Ptr ptr) False)
                        (t_hrs_' (globals x))\<rparr>\<rparr>) \<in> rf_sr"
   (is "\<forall>\<sigma> x. ?P \<sigma> x \<longrightarrow>
     (\<sigma>\<lparr>ksPSpace := ?ks \<sigma>\<rparr>, x\<lparr>globals := globals x\<lparr>t_hrs_' := ?ks' x\<rparr>\<rparr>) \<in> rf_sr")
 proof (intro impI allI)
+  define array_len where "array_len \<equiv> pt_array_len"
+  note array_len_def = pt_array_len_def array_len_def
+
   fix \<sigma> x
   let ?thesis = "(\<sigma>\<lparr>ksPSpace := ?ks \<sigma>\<rparr>, x\<lparr>globals := globals x\<lparr>t_hrs_' := ?ks' x\<rparr>\<rparr>) \<in> rf_sr"
   let ?ks = "?ks \<sigma>"
   let ?ks' = "?ks' x"
-  let ?ptr = "Ptr ptr :: (pte_C[512]) ptr"
+  let ?ptr = "pt_Ptr ptr"
   assume "?P \<sigma> x"
   hence rf: "(\<sigma>, x) \<in> rf_sr"
     and cover: "range_cover ptr sz (ptBits pt_t) 1"
@@ -1983,9 +1987,9 @@ proof (intro impI allI)
     and pal: "pspace_aligned' \<sigma>"
     and pdst: "pspace_distinct' \<sigma>"
     and pno: "pspace_no_overlap' ptr sz \<sigma>"
-    and rzo: "ret_zero ptr (2 ^ (ptBits pt_t)) \<sigma>"
-    and empty: "region_is_bytes ptr (2 ^ (ptBits pt_t)) x"
-    and zero: "heap_list_is_zero (hrs_mem (t_hrs_' (globals x))) ptr (2 ^ (ptBits pt_t))"
+    and rzo: "ret_zero ptr (2 ^ ptBits pt_t) \<sigma>"
+    and empty: "region_is_bytes ptr (2 ^ ptBits pt_t) x"
+    and zero: "heap_list_is_zero (hrs_mem (t_hrs_' (globals x))) ptr (2 ^ ptBits pt_t)"
     and kernel_data_refs_disj : "kernel_data_refs \<inter> {ptr..+ 2 ^ (ptBits pt_t)} = {}"
     by (clarsimp simp:range_cover_def[where 'a=machine_word_len, folded word_bits_def])+
 
@@ -1993,7 +1997,8 @@ proof (intro impI allI)
           Int_atLeastAtMost atLeastatMost_empty_iff split_paired_Ex
 
   (* obj specific *)
-  have mko: "\<And>dev. makeObjectKO dev (Inr AARCH64_H.PageTableObject) = Some ko" by (simp add: ko_def makeObjectKO_def)
+  have mko: "\<And>dev. makeObjectKO dev (Inr AARCH64_H.PageTableObject) = Some ko"
+    by (simp add: ko_def makeObjectKO_def)
 
   have relrl:
     "cpte_relation makeObject (from_bytes (replicate (size_of TYPE(pte_C)) 0))"
@@ -2003,9 +2008,9 @@ proof (intro impI allI)
     apply (simp add: from_bytes_def)
     apply (simp add: typ_info_simps pte_C_tag_def pte_lift_def
                      size_td_lt_final_pad size_td_lt_ti_typ_pad_combine Let_def size_of_def)
-    apply (simp add: final_pad_def Let_def size_td_lt_ti_typ_pad_combine Let_def
+    apply (simp add: final_pad_def Let_def size_td_lt_ti_typ_pad_combine
                      size_of_def padup_def align_td_array' size_td_array update_ti_adjust_ti
-                     ti_typ_pad_combine_def Let_def ti_typ_combine_def empty_typ_info_def)
+                     ti_typ_pad_combine_def ti_typ_combine_def empty_typ_info_def)
     apply (simp add: typ_info_array array_tag_def eval_nat_numeral)
     apply (simp add: array_tag_n.simps)
     apply (simp add: final_pad_def size_td_lt_ti_typ_pad_combine Let_def
@@ -2017,37 +2022,31 @@ proof (intro impI allI)
   (* /obj specific *)
 
   (* s/obj/obj'/ *)
-  (* FIXME AARCH64 need to figure out something better than shoving pt_t in
-  have szo: "size_of TYPE(pte_C[512]) = 2 ^ (ptBits pt_t)"
-    by (simp add: size_of_def size_td_array bit_simps)
-  have szo2: "512 * size_of TYPE(pte_C) = 2 ^ (ptBits pt_t)"
-    by (simp add: szo[symmetric] bit_simps) *)
+  have szo: "size_of TYPE(pte_C[pt_array_len]) = 2 ^ ptBits pt_t"
+    by (simp add: size_of_def size_td_array bit_simps pt_t_def)
+  have szo2[unfolded array_len_def]: "array_len * size_of TYPE(pte_C) = 2 ^ ptBits pt_t"
+    by (simp add: szo[symmetric] bit_simps pt_t_def array_len_def)
   have szo': "size_of TYPE(pte_C) = 2 ^ objBitsKO ko"
-    by (simp add: objBits_simps ko_def archObjSize_def bit_simps)
+    by (simp add: objBits_simps ko_def bit_simps)
 
-  (* FIXME AARCH64
   note rl' = cslift_ptr_retyp_other_inst[where n=1,
     simplified, OF empty, simplified, OF cover[simplified]
-    szo[symmetric] szo[simplified bit_simps_corres]] *)
+    szo[symmetric] szo[simplified bit_simps_corres]]
 
-  have sz_weaken: "objBitsKO ko \<le> (ptBits pt_t)" (* FIXME AARCH64 might want pt_t generic here *)
-    by (simp add: objBits_simps ko_def archObjSize_def bit_simps)
-  (* FIXME AARCH64 512
-  have cover': "range_cover ptr sz (objBitsKO ko) 512"
+  have sz_weaken: "objBitsKO ko \<le> ptBits pt_t"
+    by (simp add: objBits_simps ko_def bit_simps)
+  have cover'[unfolded array_len_def]: "range_cover ptr sz (objBitsKO ko) array_len"
     apply (rule range_cover_rel[OF cover sz_weaken])
-    apply (simp add: ptBits_def objBits_simps ko_def archObjSize_def bit_simps)
-    done *)
+    apply (simp add: ptBits_def objBits_simps ko_def bit_simps pt_t_def array_len_def)
+    done
   from sz sz_weaken have sz': "objBitsKO ko \<le> sz" by simp
   note al' = is_aligned_weaken[OF al sz_weaken]
 
   have koT: "koTypeOf ko = ArchT PTET"
     by (simp add: ko_def)
 
-  (* rest used to be generic, but PT arrays are complicating everything *)
-
-  (* FIXME AARCH64
   note rl = projectKO_opt_retyp_other [OF cover' pal pno ko_def]
-  note cterl = retype_ctes_helper [OF pal pdst pno al' sz' szb mko cover'] *)
+  note cterl = retype_ctes_helper [OF pal pdst pno al' sz' szb mko cover']
 
   have guard: "c_guard ?ptr"
     using al[simplified bit_simps]
@@ -2056,90 +2055,241 @@ proof (intro impI allI)
     apply (simp_all add:  align_td_array align_of_def bit_simps ptr0 split: if_split)
     done
 
-  (* FIXME AARCH64 512
-  have guard': "\<forall>n < 512. c_guard (pte_Ptr ptr +\<^sub>p int n)"
+  have guard'[unfolded array_len_def]: "\<forall>n < array_len. c_guard (pte_Ptr ptr +\<^sub>p int n)"
+    unfolding array_len_def
     using al[simplified bit_simps]
     apply -
     apply (rule retype_guard_helper [OF cover' ptr0 szo', where m=3])
-     apply (simp_all add: objBits_simps ko_def archObjSize_def align_of_def bit_simps)
-    done *)
+     apply (simp_all add: objBits_simps ko_def align_of_def bit_simps)
+    done
 
   note ptr_retyps.simps[simp del]
 
   from rf have pterl: "cmap_relation (map_to_ptes (ksPSpace \<sigma>)) (cslift x) Ptr cpte_relation"
     unfolding rf_sr_def cstate_relation_def by (simp add: Let_def cpspace_relation_def)
 
-  (* FIXME AARCH64
   note ht_rl = clift_eq_h_t_valid_eq[OF rl', OF tag_disj_via_td_name, simplified]
     uinfo_array_tag_n_m_not_le_typ_name
 
-  have pte_arr: "cpspace_pte_array_relation (ksPSpace \<sigma>) (t_hrs_' (globals x))
-    \<Longrightarrow> cpspace_pte_array_relation ?ks ?ks'"
-   apply (erule cmap_relation_array_add_array[OF _ al])
-        apply (simp add: foldr_upd_app_if[folded data_map_insert_def])
-        apply (rule projectKO_opt_retyp_same, simp add: ko_def projectKOs)
-       apply (simp add: h_t_valid_clift_Some_iff dom_def split: if_split)
-       apply (subst clift_ptr_retyps_gen_prev_memset_same[where n=1, simplified, OF guard],
-         simp_all only: szo refl empty, simp_all add: zero[simplified])[1]
-        apply (simp add: bit_simps word_bits_def)
-       apply (auto split: if_split)[1]
-      apply (simp_all add: objBits_simps archObjSize_def bit_simps
-                           ko_def word_bits_def)
-   done
+  have ptTranslationBits_num[unfolded array_len_def]:
+    "2 ^ ptTranslationBits pt_t = array_len"
+    by (simp add: bit_simps array_len_def pt_t_def)
 
   from rf have "cpspace_relation (ksPSpace \<sigma>) (underlying_memory (ksMachineState \<sigma>)) (t_hrs_' (globals x))"
     unfolding rf_sr_def cstate_relation_def by (simp add: Let_def)
   hence "cpspace_relation ?ks (underlying_memory (ksMachineState \<sigma>))  ?ks'"
     unfolding cpspace_relation_def
-    using pte_arr
     supply image_cong_simp [cong del]
-    apply (clarsimp simp: rl' cterl cte_C_size tag_disj_via_td_name
+    apply (clarsimp simp: rl' cterl cte_C_size tag_disj_via_td_name ptTranslationBits_num
                           foldr_upd_app_if [folded data_map_insert_def])
     apply (simp add: ptr_retyp_to_array[simplified])
     apply (subst clift_ptr_retyps_gen_prev_memset_same[OF guard'], simp_all only: szo2 empty)
        apply simp
-      apply (simp(no_asm) add: bit_simps word_bits_def)
+      apply (simp(no_asm) add: bit_simps word_bits_def pt_t_def)
      apply (simp add: zero[simplified])
-    apply (simp add: rl projectKOs del: pte_C_size)
-    apply (simp add: rl projectKO_opt_retyp_same ko_def projectKOs Let_def
+    apply (simp add: rl del: pte_C_size)
+    apply (simp add: rl projectKO_opt_retyp_same ko_def Let_def
                      ptr_add_to_new_cap_addrs [OF szo']
                 cong: if_cong del: pte_C_size)
     apply (erule cmap_relation_retype)
     apply (insert relrl, auto)
     done
 
-  moreover
-  from rf szb al
-  have "ptr_span (pt_Ptr (symbol_table ''kernel_root_pageTable'')) \<inter> {ptr ..+ 2 ^ ptBits} = {}"
-    apply (clarsimp simp: valid_global_refs'_def  Let_def
-                          valid_refs'_def ran_def rf_sr_def cstate_relation_def)
-    apply (erule disjoint_subset)
-    apply (simp add:kernel_data_refs_disj[simplified bit_simps_corres])
-    done
-
-  ultimately *)
-  show ?thesis using rf empty kernel_data_refs_disj rzo
-    sorry (* FIXME AARCH64 proof needs rework for AArch64 different table types
+  with rf empty kernel_data_refs_disj rzo
+  show ?thesis
     apply (simp add: rf_sr_def cstate_relation_def Let_def rl' tag_disj_via_td_name)
     apply (simp add: carch_state_relation_def cmachine_state_relation_def)
-    apply (clarsimp simp add: rl' cterl tag_disj_via_td_name
-      hrs_htd_update ht_rl foldr_upd_app_if [folded data_map_insert_def] rl projectKOs
-      cvariable_array_ptr_retyps[OF szo]
-      zero_ranges_ptr_retyps[where p="pt_Ptr ptr", simplified szo])
+    apply (clarsimp simp: rl' cterl tag_disj_via_td_name pt_t_def bit_simps
+                          hrs_htd_update ht_rl foldr_upd_app_if [folded data_map_insert_def] rl
+                          cvariable_array_ptr_retyps[OF szo]
+                          zero_ranges_ptr_retyps[where p="pt_Ptr ptr", simplified szo])
     apply (subst h_t_valid_ptr_retyps_gen_disjoint, assumption)
      apply (simp add:szo cte_C_size cte_level_bits_def)
      apply (erule disjoint_subset)
-     apply (simp add: bit_simps del: replicate_numeral)
+     apply (simp add: pt_t_def bit_simps del: replicate_numeral)
     apply (subst h_t_valid_ptr_retyps_gen_disjoint, assumption)
      apply (simp add:szo cte_C_size cte_level_bits_def)
      apply (erule disjoint_subset)
-     apply (simp add: bit_simps del: replicate_numeral)
-    by (simp add:szo ptr_retyps_htd_safe_neg hrs_htd_def
-      kernel_data_refs_domain_eq_rotate bit_simps
-      Int_ac del: replicate_numeral) *)
+     apply (simp add: pt_t_def bit_simps del: replicate_numeral)
+    apply (simp add: szo ptr_retyps_htd_safe_neg hrs_htd_def Int_ac
+                     kernel_data_refs_domain_eq_rotate bit_simps
+                del: replicate_numeral)
+    done
 
 qed
 
+lemma createObjects_ccorres_pte_vs:
+  defines "ko \<equiv> (KOArch (KOPTE (makeObject :: pte)))"
+  (* see createObjects_ccorres_pte_pt why this can't be generic *)
+  defines "pt_t \<equiv> VSRootPT_T"
+  shows "\<forall>\<sigma> x. (\<sigma>, x) \<in> rf_sr \<and> ptr \<noteq> 0
+  \<and> pspace_aligned' \<sigma> \<and> pspace_distinct' \<sigma>
+  \<and> pspace_no_overlap' ptr sz \<sigma>
+  \<and> ret_zero ptr (2 ^ (ptBits pt_t)) \<sigma>
+  \<and> region_is_zero_bytes ptr (2 ^ (ptBits pt_t)) x
+  \<and> range_cover ptr sz (ptBits pt_t) 1
+  \<and> valid_global_refs' s
+  \<and> kernel_data_refs \<inter> {ptr..+ 2 ^ (ptBits pt_t) } = {} \<longrightarrow>
+  (\<sigma>\<lparr>ksPSpace := foldr (\<lambda>addr. data_map_insert addr ko)
+                       (new_cap_addrs (2 ^ (ptTranslationBits pt_t)) ptr ko) (ksPSpace \<sigma>)\<rparr>,
+   x\<lparr>globals := globals x
+                 \<lparr>t_hrs_' := hrs_htd_update (ptr_retyps_gen 1 (vs_Ptr ptr) False)
+                       (t_hrs_' (globals x))\<rparr>\<rparr>) \<in> rf_sr"
+  (is "\<forall>\<sigma> x. ?P \<sigma> x \<longrightarrow>
+    (\<sigma>\<lparr>ksPSpace := ?ks \<sigma>\<rparr>, x\<lparr>globals := globals x\<lparr>t_hrs_' := ?ks' x\<rparr>\<rparr>) \<in> rf_sr")
+proof (intro impI allI)
+  define array_len where "array_len \<equiv> vs_array_len"
+  note array_len_def = vs_array_len_def array_len_def
+
+  fix \<sigma> x
+  let ?thesis = "(\<sigma>\<lparr>ksPSpace := ?ks \<sigma>\<rparr>, x\<lparr>globals := globals x\<lparr>t_hrs_' := ?ks' x\<rparr>\<rparr>) \<in> rf_sr"
+  let ?ks = "?ks \<sigma>"
+  let ?ks' = "?ks' x"
+  let ?ptr = "vs_Ptr ptr"
+  assume "?P \<sigma> x"
+  hence rf: "(\<sigma>, x) \<in> rf_sr"
+    and cover: "range_cover ptr sz (ptBits pt_t) 1"
+    and al: "is_aligned ptr (ptBits pt_t)"
+    and ptr0: "ptr \<noteq> 0"
+    and sz: "(ptBits pt_t) \<le> sz"
+    and szb: "sz < word_bits"
+    and pal: "pspace_aligned' \<sigma>"
+    and pdst: "pspace_distinct' \<sigma>"
+    and pno: "pspace_no_overlap' ptr sz \<sigma>"
+    and rzo: "ret_zero ptr (2 ^ ptBits pt_t) \<sigma>"
+    and empty: "region_is_bytes ptr (2 ^ ptBits pt_t) x"
+    and zero: "heap_list_is_zero (hrs_mem (t_hrs_' (globals x))) ptr (2 ^ ptBits pt_t)"
+    and kernel_data_refs_disj : "kernel_data_refs \<inter> {ptr..+ 2 ^ (ptBits pt_t)} = {}"
+    by (clarsimp simp:range_cover_def[where 'a=machine_word_len, folded word_bits_def])+
+
+    note blah[simp del] =  atLeastAtMost_iff atLeastatMost_subset_iff atLeastLessThan_iff
+          Int_atLeastAtMost atLeastatMost_empty_iff split_paired_Ex
+
+  (* obj specific *)
+  have mko: "\<And>dev. makeObjectKO dev (Inr AARCH64_H.PageTableObject) = Some ko"
+    by (simp add: ko_def makeObjectKO_def)
+
+  have relrl:
+    "cpte_relation makeObject (from_bytes (replicate (size_of TYPE(pte_C)) 0))"
+    unfolding cpte_relation_def
+    supply if_cong[cong]
+    apply (simp add: Let_def makeObject_pte size_of_def pte_lift_def)
+    apply (simp add: from_bytes_def)
+    apply (simp add: typ_info_simps pte_C_tag_def pte_lift_def
+                     size_td_lt_final_pad size_td_lt_ti_typ_pad_combine Let_def size_of_def)
+    apply (simp add: final_pad_def Let_def size_td_lt_ti_typ_pad_combine
+                     size_of_def padup_def align_td_array' size_td_array update_ti_adjust_ti
+                     ti_typ_pad_combine_def ti_typ_combine_def empty_typ_info_def)
+    apply (simp add: typ_info_array array_tag_def eval_nat_numeral)
+    apply (simp add: array_tag_n.simps)
+    apply (simp add: final_pad_def size_td_lt_ti_typ_pad_combine Let_def
+                     size_of_def padup_def align_td_array' size_td_array update_ti_adjust_ti
+                     ti_typ_pad_combine_def ti_typ_combine_def empty_typ_info_def)
+    apply (simp add: update_ti_t_machine_word_0s pte_get_tag_def pte_tag_defs)
+    done
+
+  (* /obj specific *)
+
+  (* s/obj/obj'/ *)
+  have szo: "size_of TYPE(pte_C[vs_array_len]) = 2 ^ ptBits pt_t"
+    by (simp add: size_of_def size_td_array pt_bits_def table_size_def pt_t_def
+                  ptTranslationBits_vs_array_len power_add pte_bits_def word_size_bits_def)
+  have szo2[unfolded array_len_def]: "array_len * size_of TYPE(pte_C) = 2 ^ ptBits pt_t"
+    by (simp add: szo[symmetric] pt_bits_def table_size_def pt_t_def array_len_def
+                  ptTranslationBits_vs_array_len power_add pte_bits_def word_size_bits_def)
+  have szo': "size_of TYPE(pte_C) = 2 ^ objBitsKO ko"
+    by (simp add: objBits_simps ko_def bit_simps)
+
+  note rl' = cslift_ptr_retyp_other_inst[where n=1,
+    simplified, OF empty, simplified, OF cover[simplified]
+    szo[symmetric] szo[simplified bit_simps_corres]]
+
+  have sz_weaken: "objBitsKO ko \<le> ptBits pt_t"
+    by (simp add: objBits_simps ko_def bit_simps)
+  have cover'[unfolded array_len_def]: "range_cover ptr sz (objBitsKO ko) array_len"
+    apply (rule range_cover_rel[OF cover sz_weaken])
+    apply (simp add: ptBits_def objBits_simps ko_def pt_bits_def table_size_def pt_t_def
+                     array_len_def ptTranslationBits_vs_array_len)
+    done
+  from sz sz_weaken have sz': "objBitsKO ko \<le> sz" by simp
+  note al' = is_aligned_weaken[OF al sz_weaken]
+
+  have koT: "koTypeOf ko = ArchT PTET"
+    by (simp add: ko_def)
+
+  note rl = projectKO_opt_retyp_other [OF cover' pal pno ko_def]
+  note cterl = retype_ctes_helper [OF pal pdst pno al' sz' szb mko cover']
+
+  have guard: "c_guard ?ptr"
+    using al[simplified bit_simps]
+    apply -
+    apply (rule is_aligned_c_guard[where n="ptBits pt_t" and m=3])
+    apply (simp_all add:  align_td_array align_of_def bit_simps ptr0 split: if_split)
+    done
+
+  have guard'[unfolded array_len_def]: "\<forall>n < array_len. c_guard (pte_Ptr ptr +\<^sub>p int n)"
+    unfolding array_len_def
+    using al[simplified bit_simps]
+    apply -
+    apply (rule retype_guard_helper [OF cover' ptr0 szo', where m=3])
+     apply (simp_all add: objBits_simps ko_def align_of_def bit_simps)
+    done
+
+  note ptr_retyps.simps[simp del]
+
+  from rf have pterl: "cmap_relation (map_to_ptes (ksPSpace \<sigma>)) (cslift x) Ptr cpte_relation"
+    unfolding rf_sr_def cstate_relation_def by (simp add: Let_def cpspace_relation_def)
+
+  note ht_rl = clift_eq_h_t_valid_eq[OF rl', OF tag_disj_via_td_name, simplified]
+    uinfo_array_tag_n_m_not_le_typ_name
+
+  have ptTranslationBits_num[unfolded array_len_def]:
+    "2 ^ ptTranslationBits pt_t = array_len"
+    by (simp add: array_len_def pt_t_def ptTranslationBits_vs_array_len)
+
+  from rf have "cpspace_relation (ksPSpace \<sigma>) (underlying_memory (ksMachineState \<sigma>)) (t_hrs_' (globals x))"
+    unfolding rf_sr_def cstate_relation_def by (simp add: Let_def)
+  hence "cpspace_relation ?ks (underlying_memory (ksMachineState \<sigma>))  ?ks'"
+    unfolding cpspace_relation_def
+    supply image_cong_simp [cong del]
+    apply (clarsimp simp: rl' cterl cte_C_size tag_disj_via_td_name ptTranslationBits_num
+                          foldr_upd_app_if [folded data_map_insert_def])
+    apply (simp add: ptr_retyp_to_array[simplified])
+    apply (subst clift_ptr_retyps_gen_prev_memset_same[OF guard'], simp_all only: szo2 empty)
+       apply simp
+      apply (simp(no_asm) add: bit_simps word_bits_def pt_t_def split: if_split)
+     apply (simp add: zero[simplified])
+    apply (simp add: rl del: pte_C_size)
+    apply (simp add: rl projectKO_opt_retyp_same ko_def Let_def
+                     ptr_add_to_new_cap_addrs [OF szo']
+                cong: if_cong del: pte_C_size)
+    apply (erule cmap_relation_retype)
+    apply (insert relrl, auto)
+    done
+
+  with rf empty kernel_data_refs_disj rzo
+  show ?thesis
+    apply (simp add: rf_sr_def cstate_relation_def Let_def rl' tag_disj_via_td_name)
+    apply (simp add: carch_state_relation_def cmachine_state_relation_def)
+    apply (clarsimp simp: rl' cterl tag_disj_via_td_name pt_t_def ptTranslationBits_vs_array_len
+                          pt_bits_def table_size_def power_add pte_bits_def word_size_bits_def
+                          hrs_htd_update ht_rl foldr_upd_app_if [folded data_map_insert_def] rl
+                          cvariable_array_ptr_retyps[OF szo]
+                          zero_ranges_ptr_retyps[where p="pt_Ptr ptr", simplified szo])
+    apply (subst h_t_valid_ptr_retyps_gen_disjoint, assumption)
+     apply (simp add:szo cte_C_size cte_level_bits_def)
+     apply (erule disjoint_subset)
+     apply (simp del: replicate_numeral)
+    apply (subst h_t_valid_ptr_retyps_gen_disjoint, assumption)
+     apply (simp add:szo cte_C_size cte_level_bits_def)
+     apply (erule disjoint_subset)
+     apply (simp del: replicate_numeral)
+    apply (simp add: szo ptr_retyps_htd_safe_neg hrs_htd_def Int_ac
+                     kernel_data_refs_domain_eq_rotate
+                del: replicate_numeral)
+    done
+
+qed
 
 definition object_type_from_H :: "object_type \<Rightarrow> machine_word" where
   "object_type_from_H tp' \<equiv> case tp' of
@@ -3534,6 +3684,24 @@ proof -
         THEN h_t_array_valid, simplified])
     done
 
+  moreover
+  from rfsr
+  have "pt_array_relation \<sigma> (globals x)"
+    by (simp add: rf_sr_def cstate_relation_def Let_def)
+  hence "cvariable_array_map_relation (gsPTTypes (ksArchState \<sigma>))
+                                     (\<lambda>pt_t. 2 ^ ptTranslationBits pt_t)
+                                     pte_Ptr
+                                     (hrs_htd (t_hrs_' ?gs))"
+    apply (clarsimp simp: heap_updates_def)
+    apply (drule cvariable_array_ptr_retyps[OF refl, where n=1 and arr=False, simplified, rotated])
+     apply (rule empty_smaller)
+    apply (simp add: hrs_htd_update)
+    apply (erule cvariable_array_ptr_retyps[where p="tcb_cnode_Ptr (ctcb_ptr_to_tcb_ptr p)", rotated -1])
+     apply (rule refl)
+    apply simp
+    apply (rule empty_smaller[simplified])
+    done
+
   ultimately show ?thesis
     using rfsr zro'
     apply (simp add: rf_sr_def cstate_relation_def Let_def h_t_valid_clift_Some_iff
@@ -4601,17 +4769,13 @@ proof -
                      kernel_state.unfold_congs)
 qed
 
-(* FIXME AARCH64 since this uses a retype of pt_Ptr it must be NormalPT_T, but what do we do about
-   vs_Ptr? copy this lemma and adjust? In any case, this one needs rework, and adjustment of ghost
-   state updates in C *)
-lemma placeNewObject_pte:
+lemma placeNewObject_pte_pt:
   "ccorresG rf_sr \<Gamma> dc xfdc
-   ( valid_global_refs' and pspace_aligned' and pspace_distinct' and pspace_no_overlap' regionBase pageBits
+   (valid_global_refs' and pspace_aligned' and pspace_distinct' and pspace_no_overlap' regionBase pageBits
       and (\<lambda>s. 2 ^ pageBits \<le> gsMaxObjectSize s)
       and ret_zero regionBase (2 ^ pageBits)
       and K (regionBase \<noteq> 0 \<and> range_cover regionBase pageBits pageBits 1
-      \<and> ({regionBase..+2 ^ pageBits} \<inter> kernel_data_refs = {})
-      ))
+      \<and> ({regionBase..+2 ^ pageBits} \<inter> kernel_data_refs = {})))
     ({s. region_actually_is_zero_bytes regionBase (2 ^ pageBits) s})
     hs
     (placeNewObject regionBase (makeObject :: pte) (ptTranslationBits NormalPT_T))
@@ -4633,11 +4797,10 @@ lemma placeNewObject_pte:
   apply (subgoal_tac "region_is_bytes regionBase 4096 x")
    apply (rule bexI [OF _ placeNewObject_eq])
       apply (clarsimp simp: split_def new_cap_addrs_def)
-      apply (cut_tac s=\<sigma> in createObjects_ccorres_pte [where ptr=regionBase and sz=pageBits])
-      sorry (* FIXME AARCH64 rework needed from createObjects_ccorres_pte
+      apply (cut_tac s=\<sigma> in createObjects_ccorres_pte_pt [where ptr=regionBase and sz=pageBits])
       apply (erule_tac x=\<sigma> in allE, erule_tac x=x in allE)
       apply (clarsimp elim!: is_aligned_weaken simp: objBitsKO_def word_bits_def)+
-      apply (clarsimp simp: split_def objBitsKO_def archObjSize_def
+      apply (clarsimp simp: objBitsKO_def archObjSize_def
                             rf_sr_def split_def Let_def ptr_retyps_gen_def
                             new_cap_addrs_def field_simps power_add
                       cong: globals.unfold_congs)
@@ -4646,7 +4809,65 @@ lemma placeNewObject_pte:
     apply (clarsimp simp: objBitsKO_def range_cover.aligned archObjSize_def bit_simps)
    apply (clarsimp simp: no_fail_def)
   apply (simp add: region_actually_is_bytes bit_simps)
- done *)
+  done
+
+(* FIXME AARCH64: move; could be simp *)
+lemma pt_bits_minus_pte_bits:
+  "pt_bits pt_t - pte_bits = ptTranslationBits pt_t"
+  by (simp add: bit_simps)
+
+(* FIXME AARCH64: move; could be simp *)
+lemma ptTranslationBits_plus_pte_bits:
+  "ptTranslationBits pt_t + pte_bits = pt_bits pt_t"
+  by (simp add: bit_simps)
+
+lemma placeNewObject_pte_vs:
+  "ccorresG rf_sr \<Gamma> dc xfdc
+   (valid_global_refs' and pspace_aligned' and pspace_distinct'
+      and pspace_no_overlap' regionBase (pt_bits VSRootPT_T)
+      and (\<lambda>s. 2 ^ pt_bits VSRootPT_T \<le> gsMaxObjectSize s)
+      and ret_zero regionBase (2 ^ pt_bits VSRootPT_T)
+      and K (regionBase \<noteq> 0 \<and> range_cover regionBase (pt_bits VSRootPT_T) (pt_bits VSRootPT_T) 1
+      \<and> ({regionBase..+2 ^ pt_bits VSRootPT_T} \<inter> kernel_data_refs = {})))
+    ({s. region_actually_is_zero_bytes regionBase (2 ^ pt_bits VSRootPT_T) s})
+    hs
+    (placeNewObject regionBase (makeObject :: pte) (ptTranslationBits VSRootPT_T))
+    (global_htd_update (\<lambda>_. (ptr_retyp (vs_Ptr regionBase))))"
+  apply (rule ccorres_from_vcg_nofail)
+  apply clarsimp
+  apply (rule conseqPre)
+  apply vcg
+  apply (clarsimp simp: rf_sr_htd_safe)
+  apply (intro conjI allI impI)
+   apply (clarsimp simp: rf_sr_def cstate_relation_def Let_def
+                         kernel_data_refs_domain_eq_rotate)
+   apply (erule ptr_retyp_htd_safe_neg)
+    apply (simp add: pt_bits_def table_size_def power_add ptTranslationBits_vs_array_len)
+    apply (simp add: bit_simps)
+   apply simp
+  apply (frule range_cover_rel[where sbit' = pte_bits])
+    apply (simp add: bit_simps split: if_split)
+   apply (rule refl)
+  apply (frule range_cover.unat_of_nat_shift[where gbits = 3 ])
+    apply (simp add: bit_simps)
+   apply (rule le_refl)
+  apply (subgoal_tac "region_is_bytes regionBase (2 ^ pt_bits VSRootPT_T) x")
+   apply (rule bexI [OF _ placeNewObject_eq])
+      apply (clarsimp simp: split_def new_cap_addrs_def)
+      apply (cut_tac s=\<sigma> in createObjects_ccorres_pte_vs[where ptr=regionBase and sz="pt_bits VSRootPT_T"])
+      apply (erule_tac x=\<sigma> in allE, erule_tac x=x in allE)
+      apply (clarsimp elim!: is_aligned_weaken simp: objBitsKO_def word_bits_def)+
+      apply (clarsimp simp: objBitsKO_def archObjSize_def pt_bits_minus_pte_bits
+                            rf_sr_def split_def Let_def ptr_retyps_gen_def
+                            new_cap_addrs_def field_simps power_add
+                      cong: globals.unfold_congs)
+      apply (simp add: Int_ac)
+     apply (clarsimp simp: word_bits_conv range_cover_def archObjSize_def)
+    apply (clarsimp simp: objBitsKO_def range_cover.aligned archObjSize_def
+                          ptTranslationBits_plus_pte_bits)
+   apply (clarsimp simp: no_fail_def)
+  apply (simp add: region_actually_is_bytes bit_simps)
+  done
 
 (* FIXME move *)
 lemma dom_disj_union:
@@ -5477,8 +5698,19 @@ proof -
     apply (simp add: projectKO_opt_retyp_other' objBitsKO_vcpu cl_vcpu)
     done
 
+  from sr
+  have "pt_array_relation \<sigma> (globals \<sigma>')"
+    by (simp add: rf_sr_def cstate_relation_def Let_def)
+  hence pt_array:
+    "cvariable_array_map_relation (gsPTTypes (ksArchState \<sigma>))
+                                  (\<lambda>pt_t. 2 ^ ptTranslationBits pt_t)
+                                  pte_Ptr
+                                  (hrs_htd ?htdret)"
+    using is_bytes cvariable_array_ptr_retyps[where n=1 and p="vcpu_Ptr p" and arr=False]
+    by (fastforce simp add: hrs_htd_update ptr_retyps_gen_def)
+
   show ?thesis
-    using assms zro' csrel' arel csrel map_vcpus
+    using assms zro' csrel' arel csrel map_vcpus pt_array
     apply (clarsimp simp: ko_vcpu_def vcpu0_def)
     apply (clarsimp simp: rf_sr_def cstate_relation_def carch_state_relation_def
                           cmachine_state_relation_def Let_def h_t_valid_clift_Some_iff)
@@ -5603,6 +5835,27 @@ lemma canonical_address_and_maskD:
   apply fastforce
   done
 
+lemma updatePTType_ccorres:
+  "ccorres dc xfdc
+           \<top>
+           {s. h_t_array_valid (hrs_htd (t_hrs_' (globals s)))
+                               (pte_Ptr regionBase)
+                               (2 ^ ptTranslationBits pt_t)}
+           hs
+           (updatePTType regionBase pt_t)
+           (Basic (globals_update (ghost'state_'_update (gs_new_pt_t pt_t regionBase))))"
+  apply (rule ccorres_from_vcg)
+  apply vcg_step
+  apply (clarsimp simp: updatePTType_def simpler_gets_def simpler_modify_def bind_def return_def)
+  apply (case_tac "ghost'state_' (globals x)")
+  apply (clarsimp simp: rf_sr_def cstate_relation_def Let_def fun_upd_def
+                        carch_state_relation_def cmachine_state_relation_def
+                        gs_new_pt_t_def ghost_size_rel_def carch_globals_def
+                        ghost_assertion_data_get_def
+                  cong: if_cong)
+  apply (clarsimp simp: cvariable_array_map_relation_def split: if_splits)
+  done
+
 (* FIXME AARCH64 multiple issues in vspace objects, possibly missing ghost state updates, and
    page table ghost state in state relation *)
 lemma Arch_createObject_ccorres:
@@ -5670,19 +5923,57 @@ subgoal
                    placeNewDataObject_ccorres[where us=18 and newType=newType, simplified]
                    gsUserPages_update_ccorres[folded modify_gsUserPages_update])
            | (rule match_ccorres, csymbr))+)[1]
-       sorry (* FIXME AARCH64
        apply (intro conjI)
         apply (clarsimp simp: createObject_hs_preconds_def frameSizeConstants_defs ptTranslationBits_def
                               APIType_capBits_def pageBits_def)
        apply (clarsimp simp: pageBits_def ccap_relation_def APIType_capBits_def
                    framesize_to_H_def cap_to_H_simps cap_frame_cap_lift
                    vm_page_size_defs ptTranslationBits_def
-                   vmrights_to_H_def mask_def vm_rights_defs c_valid_cap_def cl_valid_cap_def)  *)
-
+                   canonical_address_and_maskD[unfolded mask_def, simplified]
+                   vmrights_to_H_def mask_def vm_rights_defs c_valid_cap_def cl_valid_cap_def)
+  done
       apply (in_case "VSpaceObject")
-subgoal
-  (* FIXME AARCH64 TODO *)
-sorry
+  subgoal
+    apply (cinit' lift: t_' regionBase_' userSize_' deviceMemory_')
+     apply (simp add: object_type_from_H_def Kernel_C_defs)
+     apply (simp add: ccorres_cond_univ_iff ccorres_cond_empty_iff asidInvalid_def
+                      sle_positive APIType_capBits_def shiftL_nat objBits_simps
+                      ptBits_def pageBits_def word_sle_def word_sless_def)
+     apply (rule ccorres_rhs_assoc)+
+     apply (clarsimp simp: hrs_htd_update bitSimps objBits_simps
+                           AARCH64_H.createObject_def pt_bits_minus_pte_bits)
+     apply (ctac pre only: add: placeNewObject_pte_vs[simplified])
+       apply (ctac only: add: updatePTType_ccorres)
+         apply csymbr
+         apply (rule ccorres_return_C)
+           apply simp
+          apply simp
+         apply simp
+        apply wp
+       apply vcg
+      apply wp
+     apply vcg
+    apply clarify
+    apply (intro conjI)
+     apply (clarsimp simp: invs_pspace_aligned' invs_pspace_distinct' invs_valid_global'
+                           APIType_capBits_def invs_queues invs_valid_objs'
+                           invs_urz)
+    apply clarsimp
+    apply (clarsimp simp: ccap_relation_def APIType_capBits_def
+                          framesize_to_H_def cap_to_H_simps cap_vspace_cap_lift
+                          vmrights_to_H_def isFrameType_def canonical_address_and_maskD)
+    apply (prop_tac "c_guard (vs_Ptr regionBase)")
+     apply (rule is_aligned_c_guard[where m=pte_bits], simp, simp)
+       apply (simp add: align_of_array)
+       apply (simp add: align_of_def bit_simps)
+      apply (simp add: bit_simps split: if_split)
+     apply (simp add: bit_simps)
+    apply (drule_tac p="vs_Ptr regionBase" and
+                     d="hrs_htd (t_hrs_' (globals s'))" and
+                     g="c_guard" in ptr_retyp_h_t_valid)
+    apply (drule h_t_array_valid)
+    apply (simp add: hrs_htd_update ptTranslationBits_vs_array_len)
+    done
 
       apply (in_case "SmallPageObject")
 subgoal
@@ -5700,14 +5991,14 @@ subgoal
                 placeNewDataObject_ccorres[where us=0 and newType=newType, simplified]
                 gsUserPages_update_ccorres[folded modify_gsUserPages_update])
         | (rule match_ccorres, csymbr))+)[1]
-      sorry (* FIXME AARCH64
       apply (intro conjI)
        apply (clarsimp simp: createObject_hs_preconds_def frameSizeConstants_defs
                             APIType_capBits_def pageBits_def)
-       apply (clarsimp simp: pageBits_def ccap_relation_def APIType_capBits_def
-                 framesize_to_H_def cap_to_H_simps cap_frame_cap_lift vm_page_size_defs
-                 vmrights_to_H_def mask_def vm_rights_defs c_valid_cap_def cl_valid_cap_def) *)
-
+       apply (clarsimp simp: pageBits_def ccap_relation_def APIType_capBits_def cl_valid_cap_def
+                             framesize_to_H_def cap_to_H_simps cap_frame_cap_lift vm_page_size_defs
+                             canonical_address_and_maskD[unfolded mask_def, simplified]
+                             vmrights_to_H_def mask_def vm_rights_defs c_valid_cap_def)
+  done
      apply (in_case "LargePageObject")
 subgoal
      apply (cinit' lift: t_' regionBase_' userSize_' deviceMemory_')
@@ -5719,7 +6010,6 @@ subgoal
                             pageBits_def ptTranslationBits_def cond_second_eq_seq_ccorres
                             modify_gsUserPages_update
                       intro!: ccorres_rhs_assoc)
-      sorry (* FIXME AARCH64
       apply ((rule ccorres_return_C | simp | wp | vcg
         | (rule match_ccorres, ctac add:
                 placeNewDataObject_ccorres[where us=9 and newType=newType, simplified]
@@ -5731,38 +6021,56 @@ subgoal
       apply (clarsimp simp: pageBits_def ccap_relation_def APIType_capBits_def
                             framesize_to_H_def cap_to_H_simps cap_frame_cap_lift
                             ptTranslationBits_def vm_page_size_defs vmrights_to_H_def
-                            mask_def vm_rights_defs c_valid_cap_def cl_valid_cap_def) *)
+                            canonical_address_and_maskD[unfolded mask_def, simplified]
+                            mask_def vm_rights_defs c_valid_cap_def cl_valid_cap_def)
+  done
 
     apply (in_case "PageTableObject")
+    (* FIXME AARCH64: goal here shows a vs_Ptr, but that is only because pt_Ptr and vs_Ptr are the
+                      same type in this config. Probably should get a comment at def of vs_Ptr *)
 subgoal
     apply (cinit' lift: t_' regionBase_' userSize_' deviceMemory_')
      apply (simp add: object_type_from_H_def Kernel_C_defs)
      apply (simp add: ccorres_cond_univ_iff ccorres_cond_empty_iff asidInvalid_def
                       sle_positive APIType_capBits_def shiftL_nat objBits_simps
                       ptBits_def pageBits_def word_sle_def word_sless_def)
-     sorry (* FIXME AARCH64
      apply (rule ccorres_rhs_assoc)+
      apply (clarsimp simp: hrs_htd_update bitSimps objBits_simps word_size_bits_def
                            AARCH64_H.createObject_def pageBits_def pt_bits_def table_size
                            pte_bits_def)
-     apply (ctac pre only: add: placeNewObject_pte[simplified ptTranslationBits_def])
-       apply csymbr
-       apply (rule ccorres_return_C)
+     apply (ctac pre only: add: placeNewObject_pte_pt[simplified ptTranslationBits_def, simplified])
+       apply (ctac only: add: updatePTType_ccorres)
+         apply csymbr
+         apply (rule ccorres_return_C)
+           apply simp
+          apply simp
          apply simp
-        apply simp
-       apply simp
+        apply wp
+       apply vcg
       apply wp
      apply vcg
     apply clarify
     apply (intro conjI)
      apply (clarsimp simp: invs_pspace_aligned' invs_pspace_distinct' invs_valid_global'
                            APIType_capBits_def invs_queues invs_valid_objs'
-                           invs_urz pageBits_def)
+                           invs_urz bit_simps)
     apply clarsimp
-    apply (clarsimp simp: pageBits_def ccap_relation_def APIType_capBits_def
+    apply (clarsimp simp: bit_simps ccap_relation_def APIType_capBits_def
                           framesize_to_H_def cap_to_H_simps cap_page_table_cap_lift
-                          vmrights_to_H_def isFrameType_def) *)
+                          vmrights_to_H_def isFrameType_def canonical_address_and_maskD)
+    apply (prop_tac "c_guard (pt_Ptr regionBase)")
+     apply (rule is_aligned_c_guard[where m=pte_bits], simp, simp)
+       apply (simp add: align_of_array)
+       apply (simp add: align_of_def bit_simps)
+      apply simp
+     apply (simp add: bit_simps)
+    apply (drule_tac p="pt_Ptr regionBase" and
+                     d="hrs_htd (t_hrs_' (globals s'))" and
+                     g="c_guard" in ptr_retyp_h_t_valid)
+    apply (drule h_t_array_valid)
+    apply (simp add: hrs_htd_update)
     done
+  done
 qed
 
 (* FIXME: with the current state of affairs, we could simplify gs_new_cnodes *)
@@ -6804,12 +7112,66 @@ lemma tcb_ctes_typ_region_bytes:
   apply (simp add: objBits_simps' cte_C_size)
   done
 
+
+context begin
+
+private definition "pte_bits2 = pte_bits"
+private lemma pte_bits2_num[simplified pte_bits_def bit_simps]:
+  "pte_bits2 = pte_bits" by (rule pte_bits2_def)
+
+lemma pte_bits_power_add[unfolded pte_bits2_num, simplified]:
+  "(2^pte_bits2) * 2 ^ x = (2::nat) ^ (pte_bits + x)"
+  by (simp add: power_add pte_bits2_def)
+
+end
+
+lemma pte_typ_region_bytes: (* FIXME AARCH64: should rename cnodes_retype_have_size into something more general *)
+  "\<lbrakk> cvariable_array_map_relation (gsPTTypes (ksArchState \<sigma>)) (\<lambda>x. 2^ptTranslationBits x) pte_Ptr
+                                 (hrs_htd hrs);
+     cnodes_retype_have_size {ptr..+2 ^ bits} bits
+                             (gsPTTypes (ksArchState \<sigma>) ||> (\<lambda>pt_t. ptBits pt_t - cte_level_bits));
+     0 \<notin> {ptr..+2 ^ bits}; is_aligned ptr bits;
+    clift (hrs_htd_update (typ_region_bytes ptr bits) hrs) = (clift hrs :: pte_C ptr \<Rightarrow> _) \<rbrakk>
+    \<Longrightarrow> cvariable_array_map_relation (gsPTTypes (ksArchState \<sigma>)) (\<lambda>x. 2^ptTranslationBits x)
+        pte_Ptr (typ_region_bytes ptr bits (hrs_htd hrs))"
+  apply (clarsimp simp: cvariable_array_map_relation_def h_t_array_valid_def)
+  apply (elim allE, erule impE, fastforce)
+  apply (subst valid_footprint_typ_region_bytes)
+   apply (simp add: uinfo_array_tag_n_m_def typ_uinfo_t_def typ_info_word)
+  apply (clarsimp simp: cnodes_retype_have_size_def field_simps pte_bits_power_add)
+  apply (erule allE, erule allE, erule impE, fastforce simp: in_omonad)
+  apply (clarsimp simp: pt_bits_def table_size_def)
+  apply (subst (asm) le_add_diff_inverse2, simp add: bit_simps cte_level_bits_def split: if_splits)+
+  apply (clarsimp simp add: upto_intvl_eq[symmetric] field_simps)
+  apply (case_tac "p \<in> {ptr ..+ 2 ^ bits}")
+   apply (drule h_t_array_first_element_at[where p="Ptr p" and gd=c_guard for p,
+                                           unfolded h_t_array_valid_def, simplified])
+     apply simp
+    apply (rule is_aligned_c_guard[where m=3], simp+)
+       apply clarsimp
+      apply (simp add: align_of_def)
+     apply (simp add: size_of_def power_add bit_simps split: if_split)
+    apply (simp add: bit_simps split: if_split)
+   apply (drule_tac x="pte_Ptr p" in fun_cong)
+   apply (simp add: liftt_if[folded hrs_htd_def] hrs_htd_update
+                    h_t_valid_def valid_footprint_typ_region_bytes
+             split: if_split_asm)
+   apply (subgoal_tac "p \<in> {p ..+ size_of TYPE(pte_C)}")
+    apply simp
+    apply blast
+   apply (simp add: intvl_self)
+  apply (simp only: upto_intvl_eq mask_in_range[symmetric])
+  apply (rule aligned_ranges_subset_or_disjoint_coroll; simp)
+  done
+
 lemma ccorres_typ_region_bytes_dummy:
   "ccorresG rf_sr
      AnyGamma dc xfdc
      (invs' and ct_active' and sch_act_simple and
       pspace_no_overlap' ptr bits and
-      (cnodes_retype_have_size S bits o gsCNodes)
+      (cnodes_retype_have_size S bits o gsCNodes) and
+      (\<lambda>\<sigma>. cnodes_retype_have_size S bits
+                                   (gsPTTypes (ksArchState \<sigma>) ||> (\<lambda>pt_t. ptBits pt_t-cte_level_bits)))
       and K (bits < word_bits \<and> is_aligned ptr bits \<and> 4 \<le> bits
          \<and> 0 \<notin> {ptr..+2 ^ bits}
          \<and> {ptr ..+ 2 ^ bits} \<subseteq> S
@@ -6849,13 +7211,14 @@ lemma ccorres_typ_region_bytes_dummy:
   apply (simp add: h_t_valid_clift_Some_iff)
   apply (simp add: hrs_htd_update gsCNodes_typ_region_bytes
                    cnodes_retype_have_size_mono[where T=S]
-                   tcb_ctes_typ_region_bytes[OF _ _ invs_pspace_aligned'])
+                   tcb_ctes_typ_region_bytes[OF _ _ invs_pspace_aligned']
+                   pte_typ_region_bytes o_def)
   (* FIXME AARCH64 abstraction violation, need to know config_ARM_PA_SIZE_BITS_40 is False *)
   apply (simp add: cmap_array_typ_region_bytes_triv invs_pspace_aligned' bit_simps
                    objBitsT_simps word_bits_def zero_ranges_are_zero_typ_region_bytes
                    Kernel_Config.config_ARM_PA_SIZE_BITS_40_def
              cong: conj_cong)
-  apply (rule htd_safe_typ_region_bytes, simp, blast)
+  apply (rule htd_safe_typ_region_bytes, simp (no_asm_simp), blast)
   done
 
 lemma region_is_typeless_cong:
@@ -7549,6 +7912,27 @@ lemma createObject_cnodes_have_size:
                        split: if_split_asm)
   done
 
+crunches placeNewDataObject
+  for ksArchState[wp]: "\<lambda>s. P (ksArchState s)"
+  (simp: crunch_simps)
+
+lemma createObject_cnodes_have_size_pt[unfolded o_def]:
+  "\<lbrace>\<lambda>s. is_aligned ptr (APIType_capBits newType userSize)
+      \<and> cnodes_retype_have_size R (APIType_capBits newType userSize) (gsPTTypes (ksArchState s) ||> (\<lambda>pt_t. pt_bits pt_t - cte_level_bits))\<rbrace>
+    createObject newType ptr userSize dev
+  \<lbrace>\<lambda>rv s. cnodes_retype_have_size R (APIType_capBits newType userSize) (gsPTTypes (ksArchState s) ||> (\<lambda>pt_t. pt_bits pt_t - cte_level_bits))\<rbrace>"
+  supply fun_upd_apply[simp del] fun_upd_def[symmetric, simp]
+  apply (simp add: createObject_def)
+  apply (rule hoare_pre)
+   apply (wp mapM_x_wp' | wpc | simp add: createObjects_def AARCH64_H.createObject_def updatePTType_def)+
+  apply (cases newType, simp_all add: AARCH64_H.toAPIType_def o_def)
+   apply (rule conjI, clarsimp)+
+   apply clarsimp
+  supply fun_upd_def[symmetric, simp del] fun_upd_apply[simp]
+  apply (clarsimp simp: APIType_capBits_def cnodes_retype_have_size_def bit_simps cte_level_bits_def
+                       split: if_split_asm)+
+  done
+
 lemma range_cover_not_in_neqD:
   "\<lbrakk> x \<notin> {ptr..ptr + (of_nat n << APIType_capBits newType userSize) - 1};
     range_cover ptr sz (APIType_capBits newType userSize) n; n' < n \<rbrakk>
@@ -7869,6 +8253,8 @@ shows  "ccorres dc xfdc
                   and (\<lambda>s. descendants_range_in' {ptr..(ptr && ~~ mask sz) + 2 ^ sz - 1} srcSlot (ctes_of s))
                   and cnodes_retype_have_size {ptr .. ptr + of_nat (length destSlots) * 2^ (getObjectSize newType userSize) - 1}
                       (APIType_capBits newType userSize) o gsCNodes
+                  and (\<lambda>s. cnodes_retype_have_size {ptr .. ptr + of_nat (length destSlots) * 2^ (getObjectSize newType userSize) - 1}
+                      (APIType_capBits newType userSize) (gsPTTypes (ksArchState s) ||> (\<lambda>pt_t. ptBits pt_t - cte_level_bits)))
                   and (K (srcSlot \<notin> set destSlots
                     \<and> destSlots \<noteq> []
                     \<and> range_cover ptr sz (getObjectSize newType userSize) (length destSlots)
@@ -8156,6 +8542,7 @@ shows  "ccorres dc xfdc
                   hoare_vcg_prop createObject_gsCNodes_p createObject_cnodes_have_size)
         apply (rule hoare_vcg_conj_lift[OF createObject_capRange_helper])
          apply (wp createObject_cte_wp_at' createObject_ex_cte_cap_wp_to
+                   createObject_cnodes_have_size_pt
                    createObject_no_inter[where sz = sz] hoare_vcg_all_lift hoare_weak_lift_imp)+
        apply (clarsimp simp:invs_pspace_aligned' invs_pspace_distinct' invs_valid_pspace'
          field_simps range_cover.sz conj_comms range_cover.aligned range_cover_sz'
@@ -8278,7 +8665,7 @@ shows  "ccorres dc xfdc
         createObject_hs_preconds_def range_cover.aligned range_cover_full)
    apply (frule(1) range_cover_gsMaxObjectSize, fastforce, assumption)
    apply (simp add: intvl_range_conv[OF range_cover.aligned range_cover_sz']
-                    order_trans[OF _ APIType_capBits_min])
+                    order_trans[OF _ APIType_capBits_min] o_def)
    apply (intro conjI)
            subgoal by (simp add: word_bits_def range_cover_def)
           apply (clarsimp simp:rf_sr_def cstate_relation_def Let_def)
