proof/crefine/AARCH64/Ctac_lemmas_C.thy
@@ -134,15 +134,14 @@ lemma c_guard_abs_pte:
 
 lemmas ccorres_move_c_guard_pte = ccorres_move_c_guards [OF c_guard_abs_pte]
 
-(* FIXME AARCH64: (ptBits VSRootPT_T - 3) below should be "ptTranslationsBits VSRootPT_T" instead *)
 lemma array_assertion_abs_vspace:
-  "\<forall>s s'. (s, s') \<in> rf_sr \<and> (page_table_at' VSRootPT_T pd s)
-        \<and> (n s' \<le> 2 ^ (ptBits VSRootPT_T - 3) \<and> (x s' \<noteq> 0 \<longrightarrow> n s' \<noteq> 0))
+  "\<forall>s s'. (s, s') \<in> rf_sr
+        \<and> (page_table_at' VSRootPT_T pd s \<and> gsPTTypes (ksArchState s) pd = Some VSRootPT_T)
+        \<and> (n s' \<le> 2 ^ ptTranslationBits VSRootPT_T \<and> (x s' \<noteq> 0 \<longrightarrow> n s' \<noteq> 0))
     \<longrightarrow> (x s' = 0 \<or> array_assertion (pte_Ptr pd) (n s') (hrs_htd (t_hrs_' (globals s'))))"
   apply (intro allI impI disjCI2, clarsimp)
-  apply (drule(1) vspace_at_rf_sr, clarsimp)
+  apply (drule (2) vspace_at_rf_sr, clarsimp)
   apply (erule clift_array_assertion_imp; simp)
-  apply (simp add: pt_bits_def table_size_def pte_bits_def word_size_bits_def)
   apply (rule_tac x=0 in exI, simp add: ptTranslationBits_vs_array_len)
   done
 
